reals/fast/CRexp.v
@@ -28,11 +28,19 @@ Require Import Qpower.
 Require Import COrdFields2.
 Require Import Qordfield.
 Require Import PowerSeries.
+Require Import CRpower.
+Require Import Exponential.
+Require Import RealPowers.
+Require Import Compress.
+Require Import Ndigits.
+Require Import ModulusDerivative.
+Require Import CRsign.
 Require Import CornTac.
 
 Set Implicit Arguments.
 
 Opaque CR.
+Opaque Exp.
 
 Open Local Scope Q_scope.
 
@@ -71,109 +79,6 @@ assumption.
 Defined.
 
 End ExpSeries.
-
-Lemma Qle_ZO_flip : forall a, -(1) <= a <= 0 -> 0 <= (-a) <= 1.
-Proof.
-intros a [H0 H1].
-auto with *.
-split.
-change 0 with (-0).
-apply Qopp_le_compat.
-assumption.
-change 1 with (- (-(1))).
-apply Qopp_le_compat.
-assumption.
-Qed.
-
-Definition rational_exp_small_neg (a:Q) (p:-(1) <= a <= 0) : CR 
-:= let p':= (Qle_ZO_flip p) in InfiniteAlternatingSum (expSequence_dnn p') (expSequence_zl p').
-
-Lemma rational_exp_small_neg_posH : forall (a:Q) (p:-(1) <= a <= 0),
- ('(1#3) <= rational_exp_small_neg p)%CR.
-Proof.
-intros a p.
-unfold rational_exp_small_neg.
-do 4 rewrite InfiniteAlternatingSum_step.
-generalize (dnn_tl
-                  (dnn_tl (dnn_tl (dnn_tl (expSequence_dnn (Qle_ZO_flip p)))))).
-generalize (@Limit_tl Q_as_MetricSpace
-                                (@tl Q (@tl Q (@tl Q (expSequence (Qopp a)))))
-                                (Qmake Z0 xH)
-                                (@Limit_tl Q_as_MetricSpace
-                                   (@tl Q (@tl Q (expSequence (Qopp a))))
-                                   (Qmake Z0 xH)
-                                   (@Limit_tl Q_as_MetricSpace
-                                      (@tl Q (expSequence (Qopp a)))
-                                      (Qmake Z0 xH)
-                                      (@Limit_tl Q_as_MetricSpace
-                                         (expSequence (Qopp a)) (Qmake Z0 xH)
-                                         (@expSequence_zl (Qopp a)
-                                            (@Qle_ZO_flip a p)))))).
-intros l d.
-change ('(1#3) <= '1%Q + - ('(1 * (1 * - a))%Q + - 
- ('((1 # 2) * (1 * - a * - a))%Q + - ('((1 # 6) * (1 * - a * - a * - a))%Q + 
- - InfiniteAlternatingSum d l))))%CR.
-cut ('0<=InfiniteAlternatingSum d l)%CR;[|apply InfiniteAlternatingSum_nonneg].
-generalize (InfiniteAlternatingSum d l).
-intros m Hm.
-rsapply shift_leEq_rht.
-unfold cg_minus;simpl.
-assert (X:((' 1 -
- (' (1 * (1 * - a)) -
-  (' ((1 # 2) * (1 * - a * - a)) - (' ((1 # 6) * (1 * - a * - a * - a)) - m))) -
- ' (1 # 3))==(('((1#6)*(a+1)*(1*(a+1)*(a+1)+(3#1)))%Q + m)))%CR) by (abstract ring).
-rewrite X.
-rsapply plus_resp_nonneg;[|assumption].
-rewrite CRle_Qle.
-repeat rsapply mult_resp_nonneg.
-discriminate.
-destruct p as [p _].
-rewrite Qle_minus_iff in p.
-(replace RHS with (a + - - (1)) by ring);assumption.
-rsapply plus_resp_nonneg.
-rsapply sqr_nonneg.
-discriminate.
-Qed.
-
-Lemma rational_exp_small_neg_pos : forall (a:Q) (p:-(1) <= a <= 0),
- CRpos (rational_exp_small_neg p).
-Proof.
-intros a p.
-exists (1#3)%Qpos.
-abstract (
- autorewrite with QposElim;
- rapply rational_exp_small_neg_posH).
-Defined.
-
-Definition rational_exp_small (a:Q) (p:-(1) <= a <= 1) : CR.
-intros a p.
-destruct (Qlt_le_dec_fast 0 a).
-refine (CRinv_pos (1#3) (@rational_exp_small_neg (-a) _)).
-abstract (destruct p;split;[apply Qopp_le_compat; assumption|apply (Qopp_le_compat 0); apply Qlt_le_weak; assumption]).
-apply (rational_exp_small_neg (conj (proj1 p) q)).
-Defined. 
-
-Definition E : CR.
-apply rational_exp_small with (1).
-abstract (split;discriminate).
-Defined.
-
-Section Correct.
-
-Lemma Qpower_S : forall a n, (a^S n == a*a^n).
-Proof.
-intros a n.
-destruct (Qeq_dec a 0).
-rewrite q.
-rewrite Qpower_0.
-discriminate.
-ring.
-rewrite inj_S.
-unfold Zsucc.
-rewrite Qpower_plus.
-assumption.
-ring.
-Qed.
 
 Lemma exp_ps_correct : forall a (n:nat) H, 
   inj_Q IR ((((-(1))^n)*Str_nth n (expSequence (-a)))%Q)[=]Exp_ps n (inj_Q IR a) H.
@@ -219,7 +124,10 @@ change ((1 # P_of_succ_nat n) * a * ((1 # P_of_succ_nat (pred (fac n))) * a ^ n)
 replace (P_of_succ_nat (pred (S n * fac n))%nat) with 
  (P_of_succ_nat (pred (S n)) * P_of_succ_nat (pred (fac n)))%positive.
 rewrite <- pred_Sn.
-rewrite Qpower_S.
+rewrite inj_S.
+unfold Zsucc.
+rewrite Qpower_plus'.
+auto with *.
 change ((1 # P_of_succ_nat n * P_of_succ_nat (pred (fac n))%positive))%Q
  with ((1 # P_of_succ_nat n) * (1#P_of_succ_nat (pred (fac n))))%Q.
 ring.
@@ -271,6 +179,22 @@ rapply (inj_Q_nring IR 1).
 assumption.
 Qed.
 
+Lemma Qle_ZO_flip : forall a, -(1) <= a <= 0 -> 0 <= (-a) <= 1.
+Proof.
+intros a [H0 H1].
+auto with *.
+split.
+change 0 with (-0).
+apply Qopp_le_compat.
+assumption.
+change 1 with (- (-(1))).
+apply Qopp_le_compat.
+assumption.
+Qed.
+
+Definition rational_exp_small_neg (a:Q) (p:-(1) <= a <= 0) : CR 
+:= let p':= (Qle_ZO_flip p) in InfiniteAlternatingSum (expSequence_dnn p') (expSequence_zl p').
+
 Lemma rational_exp_small_neg_correct : forall (a:Q) Ha,
  (@rational_exp_small_neg a Ha == IRasCR (Exp (inj_Q IR a)))%CR.
 Proof.
@@ -282,5 +206,447 @@ clear Ha.
 apply exp_ps_correct.
 Qed.
 
-End Correct.
+Lemma shrink_by_two : forall n a, (-(2^(S n)))%Z <= a <= 0 -> (-(2^n))%Z <= (a/2) <= 0.
+Proof.
+intros n a [H0 H1].
+split.
+ apply Qmult_lt_0_le_reg_r with 2.
+  constructor.
+ change ((-(2 ^ n)%Z) * 2 <= a / 2 * 2).
+ rewrite Zpower_Qpower.
+  auto with *.
+ rewrite (inj_S n) in H0.
+ replace LHS with (-(2%positive^n*2^1)) by ring.
+ rewrite <- Qpower_plus.
+  discriminate.
+ replace RHS with a by (field; discriminate).
+ change (- (2 ^ Zsucc n)%Z <= a) in H0.
+ rewrite Zpower_Qpower in H0.
+  assumption.
+ auto with *.
+rsapply (fun a b => mult_cancel_leEq _ a b (2:Q)).
+ constructor.
+replace LHS with a by (field; discriminate).
+replace RHS with 0 by ring.
+assumption.
+Qed.
 
+Fixpoint rational_exp_neg_bounded (n:nat) (a:Q) : (-(2^n))%Z <= a <= 0 -> CR :=
+match n return (-(2^n))%Z <= a <= 0 -> CR with
+| O => @rational_exp_small_neg a
+| S n' =>
+  match (Qlt_le_dec_fast a (-(1))) with
+  | left _ => fun H => CRpower_positive_bounded 2 (1#1) (compress (rational_exp_neg_bounded n' (shrink_by_two n' H)))
+  | right H' => fun H => rational_exp_small_neg (conj H' (proj2 H))
+  end
+end.
+
+Lemma rational_exp_neg_bounded_correct : forall n (a:Q) Ha,
+ (@rational_exp_neg_bounded n a Ha == IRasCR (Exp (inj_Q IR a)))%CR.
+Proof.
+unfold rational_exp_neg_bounded.
+induction n.
+ apply rational_exp_small_neg_correct.
+intros a Ha.
+destruct (Qlt_le_dec_fast a (- (1))).
+ rewrite IHn.
+ clear IHn.
+ rewrite compress_correct.
+ rewrite <- CRpower_positive_bounded_correct.
+  apply leEq_imp_AbsSmall.
+   apply less_leEq; apply Exp_pos.
+  stepr (One:IR).
+   apply Exp_leEq_One.
+   stepr (inj_Q IR 0) by apply (inj_Q_nring IR 0).
+   apply inj_Q_leEq.
+   apply mult_cancel_leEq with (2:Q).
+    constructor.
+   change (a/2*2<=0).
+   replace LHS with a by (field; discriminate).
+   apply Qle_trans with (-(1)); try discriminate.
+   apply Qlt_le_weak.
+   assumption. 
+  rstepl (nring 1:IR).
+  apply eq_symmetric; apply (inj_Q_nring IR 1).
+ apply IRasCR_wd.
+ set (a':=inj_Q IR (a/2)).
+ simpl. 
+ rstepl (Exp a'[*]Exp a').
+ stepl (Exp (a'[+]a')) by apply Exp_plus.
+ apply Exp_wd.
+ unfold a'.
+ eapply eq_transitive.
+  apply eq_symmetric; apply (inj_Q_plus IR).
+ apply inj_Q_wd.
+ simpl.
+ field; discriminate.
+apply rational_exp_small_neg_correct.
+Qed.
+
+Lemma rational_exp_bound_power_2 : forall (a:Q), a <= 0 -> (-2^(Z_of_nat match (Qnum a) with |Z0 => O | Zpos x => Psize x | Zneg x => Psize x end))%Z <= a.
+Proof.
+intros [[|n|n] d] Ha;
+simpl.
+  discriminate.
+ elim Ha.
+ reflexivity.
+rewrite Qle_minus_iff.
+change (0<=(-(n#d) + - (-2^Psize n)%Z)).
+rewrite Qplus_comm.
+rewrite <- Qle_minus_iff.
+change (n # d <= - - (2 ^ Psize n)%Z).
+replace RHS with ((2^Psize n)%Z:Q) by ring.
+unfold Qle.
+simpl.
+change (n * 1 <= 2 ^ Psize n * d)%Z.
+apply Zmult_le_compat; try auto with *.
+clear - n.
+apply Zle_trans with (n+1)%Z.
+ auto with *.
+induction n.
+  change (Psize (xI n)) with (1 + (Psize n))%nat.
+  rewrite inj_plus.
+  rewrite Zpower_exp; try auto with *.
+  rewrite Zpos_xI.
+  replace LHS with (2*(n+1))%Z by ring.
+  apply Zmult_le_compat; auto with *.
+ change (Psize (xO n)) with (1 + (Psize n))%nat.
+ rewrite inj_plus.
+ rewrite Zpower_exp; try auto with *.
+ rewrite Zpos_xO.
+ apply Zle_trans with (2*(n+1))%Z.
+  auto with *.
+ apply Zmult_le_compat; auto with *.
+discriminate.
+Qed.
+
+Definition rational_exp_neg (a:Q) : a <= 0 -> CR.
+intros a Ha.
+refine (@rational_exp_neg_bounded _ a _).
+split.
+ apply (rational_exp_bound_power_2 Ha).
+apply Ha.
+Defined.
+
+Lemma rational_exp_neg_correct : forall (a:Q) Ha,
+ (@rational_exp_neg a Ha == IRasCR (Exp (inj_Q IR a)))%CR.
+Proof.
+intros a Ha.
+rapply rational_exp_neg_bounded_correct.
+Qed.
+
+Lemma rational_exp_small_neg_posH : forall (a:Q) (p:-(1) <= a <= 0),
+ ('(1#3) <= rational_exp_small_neg p)%CR.
+Proof.
+intros a p.
+unfold rational_exp_small_neg.
+do 4 rewrite InfiniteAlternatingSum_step.
+generalize (dnn_tl
+                  (dnn_tl (dnn_tl (dnn_tl (expSequence_dnn (Qle_ZO_flip p)))))).
+generalize (@Limit_tl Q_as_MetricSpace
+                                (@tl Q (@tl Q (@tl Q (expSequence (Qopp a)))))
+                                (Qmake Z0 xH)
+                                (@Limit_tl Q_as_MetricSpace
+                                   (@tl Q (@tl Q (expSequence (Qopp a))))
+                                   (Qmake Z0 xH)
+                                   (@Limit_tl Q_as_MetricSpace
+                                      (@tl Q (expSequence (Qopp a)))
+                                      (Qmake Z0 xH)
+                                      (@Limit_tl Q_as_MetricSpace
+                                         (expSequence (Qopp a)) (Qmake Z0 xH)
+                                         (@expSequence_zl (Qopp a)
+                                            (@Qle_ZO_flip a p)))))).
+intros l d.
+change ('(1#3) <= '1%Q + - ('(1 * (1 * - a))%Q + - 
+ ('((1 # 2) * (1 * - a * - a))%Q + - ('((1 # 6) * (1 * - a * - a * - a))%Q + 
+ - InfiniteAlternatingSum d l))))%CR.
+cut ('0<=InfiniteAlternatingSum d l)%CR;[|apply InfiniteAlternatingSum_nonneg].
+generalize (InfiniteAlternatingSum d l).
+intros m Hm.
+rsapply shift_leEq_rht.
+unfold cg_minus;simpl.
+assert (X:((' 1 -
+ (' (1 * (1 * - a)) -
+  (' ((1 # 2) * (1 * - a * - a)) - (' ((1 # 6) * (1 * - a * - a * - a)) - m))) -
+ ' (1 # 3))==(('((1#6)*(a+1)*(1*(a+1)*(a+1)+(3#1)))%Q + m)))%CR) by (abstract ring).
+rewrite X.
+rsapply plus_resp_nonneg;[|assumption].
+rewrite CRle_Qle.
+repeat rsapply mult_resp_nonneg.
+discriminate.
+destruct p as [p _].
+rewrite Qle_minus_iff in p.
+(replace RHS with (a + - - (1)) by ring);assumption.
+rsapply plus_resp_nonneg.
+rsapply sqr_nonneg.
+discriminate.
+Qed.
+
+Lemma rational_exp_neg_posH : forall (n:nat) (a:Q) Ha, (-n <= a) ->
+ ('((1#3)^n) <= @rational_exp_neg a Ha)%CR.
+Proof.
+intros n a Ha Hn.
+rewrite rational_exp_neg_correct.
+rewrite <- IR_inj_Q_as_CR.
+rewrite <- IR_leEq_as_CR.
+stepl (inj_Q IR (1#3)[^]n) by (apply eq_symmetric; apply inj_Q_power).
+assert (X:Zero[<]inj_Q IR (1#3)).
+ stepl (inj_Q IR 0) by apply (inj_Q_nring IR 0).
+ apply inj_Q_less.
+ constructor.
+astepl (inj_Q IR (1#3)[!](nring n)[//]X).
+unfold power.
+apply Exp_resp_leEq.
+destruct n.
+ rstepl (Zero:IR).
+ stepl (inj_Q IR 0) by apply (inj_Q_nring IR 0).
+ apply inj_Q_leEq.
+ assumption.
+apply (fun a b => (shift_mult_leEq' _ a b _ (nringS_ap_zero IR n))).
+ apply nring_pos; auto with *.
+stepr (inj_Q IR (a/(S n))).
+ apply Exp_cancel_leEq.
+ astepl (inj_Q IR (1#3)).
+ rewrite IR_leEq_as_CR.
+ rewrite IR_inj_Q_as_CR.
+ assert (Ha0 : -(1)<=(a/S n)<=0).
+  split.
+   rewrite Qle_minus_iff.
+   replace RHS with ((a + S n)*(1/(S n))) by (field;discriminate).
+   replace LHS with (0*(1/(S n))) by ring.
+   rsapply mult_resp_leEq_rht.
+    replace RHS with (a + - (- (P_of_succ_nat n))) by ring.
+    rewrite <- Qle_minus_iff.
+    assumption.
+   rewrite <- (Qmake_Qdiv 1 (P_of_succ_nat n)).
+   discriminate.
+  replace RHS with (0*(1/(S n))) by ring.
+  rsapply mult_resp_leEq_rht.
+   assumption.
+  rewrite <- (Qmake_Qdiv 1 (P_of_succ_nat n)).
+  discriminate.
+ rewrite <- (rational_exp_small_neg_correct Ha0).
+ apply rational_exp_small_neg_posH.
+assert (X0:inj_Q IR (inject_Z (S n))[#]Zero).
+ stepl (inj_Q IR (nring (S n))).
+  stepl (nring (S n):IR) by (apply eq_symmetric; apply (inj_Q_nring IR (S n))).
+  apply (nringS_ap_zero).
+ apply inj_Q_wd.
+ apply nring_Q.
+stepl (inj_Q IR a[/]_[//]X0).
+ apply div_wd.
+  apply eq_reflexive.
+ stepl (inj_Q IR (nring (S n))).
+  apply inj_Q_nring.
+ apply inj_Q_wd.
+ apply nring_Q.
+apply eq_symmetric.
+apply inj_Q_div.
+Qed.
+
+Lemma rational_exp_neg_posH' : forall (a:Q) Ha,
+ ('((3#1)^(Zdiv (Qnum a) (Qden a)))%Qpos <= @rational_exp_neg a Ha)%CR.
+Proof.
+intros [n d] Ha.
+simpl.
+assert (X1:(d > 0)%Z) by auto with *.
+assert (X:n = (d * (n / d) + n mod d)%Z).
+ apply Z_div_mod_eq.
+ assumption.
+set (c:=(n/d)%Z) in *.
+assert (X0:(0 <= -c)%Z).
+ apply Zmult_le_0_reg_r with d.
+  auto with *.
+ replace RHS with (-(d*c))%Z by ring.
+ change (-(d*c))%Z with (0-(d*c))%Z.
+ rewrite <- Zle_plus_swap.
+ replace LHS with (d*c + 0)%Z by ring.
+ apply Zle_trans with n.
+  rewrite X.
+  apply Zplus_le_compat_l.
+  destruct (Z_mod_lt n _ X1).
+  assumption.
+ unfold Qle in Ha.
+ simpl in Ha.
+ replace LHS with (n*1)%Z by ring.
+ assumption.
+setoid_replace (QposAsQ ((3#1)^c)%Qpos) with ((1#3)^(Z_to_nat X0)).
+ apply rational_exp_neg_posH.
+ rewrite <- (Z_to_nat_correct X0).
+ unfold Qle.
+ simpl.
+ rewrite X.
+ replace LHS with (d*c + 0)%Z by ring.
+ replace RHS with (d*c + n mod d)%Z by ring.
+ apply Zplus_le_compat_l.
+ destruct (Z_mod_lt n _ X1).
+ assumption.
+rewrite <- Z_to_nat_correct.
+rewrite Q_Qpos_power.
+change (1#3) with (/3).
+rewrite Qinv_power.
+rewrite <- Qpower_opp.
+replace (- - c)%Z with c by ring.
+reflexivity.
+Qed.
+
+Lemma rational_exp_neg_pos : forall (a:Q) Ha,
+ CRpos (@rational_exp_neg a Ha).
+Proof.
+intros a Ha.
+exists ((3#1)^(Zdiv (Qnum a) (Qden a)))%Qpos.
+apply rational_exp_neg_posH'.
+Defined.
+
+Definition rational_exp (a:Q) : CR.
+intros a.
+destruct (Qle_total 0 a).
+refine (CRinv_pos ((3#1)^(Zdiv (Qnum (- a)) (Qden (- a))))%Qpos (@rational_exp_neg (-a) _)).
+apply (Qopp_le_compat 0); assumption.
+apply (rational_exp_neg q).
+Defined.
+
+Lemma rational_exp_correct : forall (a:Q),
+ (rational_exp a == IRasCR (Exp (inj_Q IR a)))%CR.
+Proof.
+intros a.
+unfold rational_exp.
+destruct (Qle_total 0 a); try apply rational_exp_neg_correct.
+assert (X0:=rational_exp_neg_correct (Qopp_le_compat 0 a q)).
+rewrite X0.
+assert (X:((IRasCR (Exp (inj_Q IR (- a)%Q)) >< '0)%CR)).
+ cut (rational_exp_neg (Qopp_le_compat 0 a q) >< ' 0)%CR.
+ apply CRapart_wd; assumption || reflexivity.
+ right.
+ exists ((3 # 1) ^ (Qnum (-a) / Qden (-a)))%Qpos. 
+ ring_simplify.
+ apply rational_exp_neg_posH'.
+rewrite (@CRinv_pos_inv ((3 # 1) ^ (Qnum (-a) / Qden (-a))) _ X).
+ rewrite <- X0.
+ apply rational_exp_neg_posH'.
+rewrite <- IR_recip_as_CR_2.
+apply IRasCR_wd.
+apply eq_symmetric.
+eapply eq_transitive;[|apply div_wd; apply eq_reflexive].
+apply Exp_inv'.
+rstepl ([--][--](inj_Q IR a)).
+csetoid_rewrite_rev (inj_Q_inv IR a).
+apply eq_reflexive.
+Qed.
+
+Definition CRe : CR := rational_exp 1.
+
+Lemma CRe_correct : (CRe == IRasCR E)%CR.
+Proof.
+unfold CRe.
+rewrite rational_exp_correct.
+apply IRasCR_wd.
+csetoid_replace (inj_Q IR 1) (One:IR).
+ algebra.
+rstepr (nring 1:IR).
+apply (inj_Q_nring IR 1).
+Qed.
+
+Hint Rewrite <- CRe_correct : IRtoCR.
+
+Opaque inj_Q.
+
+Definition exp_bound (z:Z) : Qpos :=
+(match z with
+ |Z0 => 1#1
+ |Zpos p => (3#1)^p
+ |Zneg p => (1#2)^p
+ end)%Qpos.
+
+(*
+Lemma exp_bound_bound : forall (z:Z) x, closer (inj_Q IR (z:Q)) x -> AbsIR (Exp x)[<=]inj_Q IR (exp_bound z:Q).
+Proof.
+intros [|z|z]; simpl; intros x Hx; 
+ apply AbsSmall_imp_AbsIR; 
+ (apply leEq_imp_AbsSmall;[apply less_leEq; apply Exp_pos|]).
+  stepr (One:IR).
+   apply Exp_leEq_One.
+   stepr (inj_Q IR (0%Z:Q)).
+    assumption.
+   apply (inj_Q_nring IR 0).
+  rstepl (nring 1:IR).
+  apply eq_symmetric; apply (inj_Q_nring IR 1).
+ stepr (Three[!](inj_Q IR (z:Q))[//](pos_three IR):IR).
+  astepl (E[!]x[//]pos_E).
+  apply real_power_resp_leEq_both.
+
+Focus 3.
+
+ try apply less_leEq;
+ apply CR_less_as_IR;
+ unfold CRlt;
+ match goal with 
+ | |- CRpos ?X => let X0 := fresh "IR_dec" in
+                  set (X0:=X);
+                  let XH := fresh "IR_dec" in
+                  assert (XH:(X==X0)%CR) by reflexivity;
+                  autorewrite with IRtoCR in XH
+ end.
+
+rewrite IR_nring_as_CR in IR_dec0.
+
+autorewrite with IRtoCR.
+ in IR_dec0.
+
+IR_nring_as_CR.
+nring
+
+:IR_solve_ineq (1#1)%Qpos.
+4:IR_solve_ineq (1#1)%Qpos.
+IR_dec_precompute.
+repeat (match goal with 
+ | H:_ |-_  => clear H
+ end).
+ match goal with 
+ | H:_ |-_  => fail 2 "Context cannot be cleared"
+ end.
+IR_solve_ineq (1#1)%Qpos.
+match goal with 
+| H:_ |-_  => clear H
+endNot satisfied with my last post, Robert 
+clear x.
+vm_compute.
+reflexivity.
+assert ((CRe - ' 1)==(CRe - ' 1))%CR.
+3:IR_dec_precompute.
+
+apply CR_epsilon_sign_dec_pos.
+exists (1#1)%Qpos.
+vm_compute.
+
+pose (X':=(CR_epsilon_sign_dec (1#1) (CRe - '1)%CR)).
+unfold CR_epsilon_sign_dec in X'.
+set (z':=(approximate (CRe - '1)%CR (1#1)%Qpos)) in X'.
+vm_compute in z'.
+unfold z' in *.
+simpl in X'.
+assert ((1#1)%Qpos < approximate (CRe - ' 1)%CR (1#1)%Qpos).
+
+
+rewrite IR_One_as_CR in XH.
+apply (CRpos_wd XH).
+
+     stepr
+  rstepl (x[*]One).
+  apply mult_resp_leEq_both.
+ 
+  
+ 
+Lemma exp_uc_prf : forall z:Z, is_UniformlyContinuousFunction (fun a => rational_exp (Qmax z a)) (exp_modulus z).
+Proof.
+intros [|z|z].
+  apply (is_UniformlyContinuousFunction_wd) with (fun a => rational_exp (Qmax 0 a)) (modulusD (1#1)).
+    reflexivity.
+   intros x; simpl.
+   autorewrite with QposElim.
+   replace RHS with (x:Q) by (field; discriminate).
+   apply Qle_refl.
+  
+  
+; simpl; intros e a b Hab.
+*)
