reals/fast/CRsign.v
@@ -1,0 +1,84 @@
+(*
+Copyright © 2006 Russell O’Connor
+
+Permission is hereby granted, free of charge, to any person obtaining a copy of
+this proof and associated documentation files (the "Proof"), to deal in
+the Proof without restriction, including without limitation the rights to
+use, copy, modify, merge, publish, distribute, sublicense, and/or sell copies of
+the Proof, and to permit persons to whom the Proof is furnished to do so,
+subject to the following conditions:
+
+The above copyright notice and this permission notice shall be included in all
+copies or substantial portions of the Proof.
+
+THE PROOF IS PROVIDED "AS IS", WITHOUT WARRANTY OF ANY KIND, EXPRESS OR
+IMPLIED, INCLUDING BUT NOT LIMITED TO THE WARRANTIES OF MERCHANTABILITY, FITNESS
+FOR A PARTICULAR PURPOSE AND NONINFRINGEMENT. IN NO EVENT SHALL THE AUTHORS OR
+COPYRIGHT HOLDERS BE LIABLE FOR ANY CLAIM, DAMAGES OR OTHER LIABILITY, WHETHER
+IN AN ACTION OF CONTRACT, TORT OR OTHERWISE, ARISING FROM, OUT OF OR IN
+CONNECTION WITH THE PROOF OR THE USE OR OTHER DEALINGS IN THE PROOF.
+*)
+
+Require Export CRIR.
+Require Import QMinMax.
+
+Definition CR_epsilon_sign_dec (e:Qpos) (x:CR) : comparison :=
+let z := (approximate x e) in
+ match (Qle_total z (2*e)) with
+ | right p => Gt
+ | left _ => 
+  match (Qle_total (-(2)*e) z) with
+  | right p => Lt
+  | left _ => Eq
+  end
+ end.
+
+Lemma CR_epsilon_sign_dec_pos : forall x, 
+{e:Qpos | CR_epsilon_sign_dec e x = Gt } -> CRpos x.
+Proof.
+intros x [e H].
+apply (@CRpos_char e).
+abstract (
+unfold CR_epsilon_sign_dec in H;
+destruct (Qle_total (approximate x e) (2 * e)) as [A|A];
+ [destruct (Qle_total (- (2) * e) (approximate x e)) as [B|B]; discriminate H|];
+assumption).
+Defined.
+
+Ltac IR_dec_precompute := 
+ try apply less_leEq;
+ apply CR_less_as_IR;
+ unfold CRlt;
+ match goal with 
+ | |- CRpos ?X => let X0 := fresh "IR_dec" in
+                  set (X0:=X);
+                  let XH := fresh "IR_dec" in
+                  assert (XH:(X==X0)%CR) by reflexivity;
+                  autorewrite with IRtoCR in XH;
+                  autorewrite with CRfast_compute in XH;
+                  apply (CRpos_wd XH);
+                  clear X0 XH
+ end.
+
+Ltac CR_solve_pos_loop e :=
+ (exists e;
+  vm_compute;
+  match goal with 
+  | |- Gt = Gt => reflexivity
+  | |- Lt = Gt => fail 2 "CR number is negative"
+  end)
+ || CR_solve_pos_loop ((1#2)*e)%Qpos.
+
+Ltac CR_solve_pos e :=
+ repeat (match goal with 
+ | H:_ |-_  => clear H
+ end);
+ match goal with 
+ | H:_ |-_  => fail 1 "Context cannot be cleared"
+ | |-_ => idtac
+ end;
+ apply CR_epsilon_sign_dec_pos;
+ CR_solve_pos_loop e.
+
+Ltac IR_solve_ineq e :=
+ IR_dec_precompute; CR_solve_pos e.
